common/Main.v
@@ -6,6 +6,8 @@ Require Import Maps.
 Require Import AST.
 Require Import Values.
 (** Languages (syntax and semantics). *)
+Require Csyntax.
+Require Csem.
 Require Csharpminor.
 Require Cminor.
 Require RTL.
@@ -14,6 +16,7 @@ Require Linear.
 Require Mach.
 Require PPC.
 (** Translation passes. *)
+Require Cshmgen.
 Require Cminorgen.
 Require RTLgen.
 Require Constprop.
@@ -24,11 +27,13 @@ Require Linearize.
 Require Stacking.
 Require PPCgen.
 (** Type systems. *)
+Require Ctyping.
 Require RTLtyping.
 Require LTLtyping.
 Require Lineartyping.
 Require Machtyping.
 (** Proofs of semantic preservation and typing preservation. *)
+Require Cshmgenproof3.
 Require Cminorgenproof.
 Require RTLgenproof.
 Require Constpropproof.
@@ -62,12 +67,9 @@ Notation "a @@ b" :=
    (apply_total _ _ a b) (at level 50, left associativity).
 
 (** We define two translation functions for whole programs: one starting with
-  a Csharpminor program, the other with a Cminor program.  Both
+  a C program, the other with a Cminor program.  Both
   translations produce PPC programs ready for pretty-printing and
-  assembling.  Some front-ends will prefer to generate Csharpminor
-  (e.g. a C front-end) while some others (e.g. an ML compiler) might
-  find it more convenient to generate Cminor directly, bypassing
-  Csharpminor.
+  assembling.  
 
   There are two ways to compose the compiler passes.  The first translates
   every function from the Cminor program from Cminor to RTL, then to LTL, etc,
@@ -89,24 +91,20 @@ Definition transf_cminor_fundef (f: Cminor.fundef) : option PPC.fundef :=
   @@@ Stacking.transf_fundef
   @@@ PPCgen.transf_fundef.
 
-(** And here is the translation for Csharpminor functions. *)
-
-Definition transf_csharpminor_fundef
-     (gce: Cminorgen.compilenv) (f: Csharpminor.fundef) : option PPC.fundef :=
-  Some f 
-  @@@ Cminorgen.transl_fundef gce
-  @@@ transf_cminor_fundef.
-
 (** The corresponding translations for whole program follow. *)
 
 Definition transf_cminor_program (p: Cminor.program) : option PPC.program :=
   transform_partial_program transf_cminor_fundef p.
 
-Definition transf_csharpminor_program (p: Csharpminor.program) : option PPC.program :=
-  let gce := Cminorgen.build_global_compilenv p in
-  transform_partial_program 
-    (transf_csharpminor_fundef gce)
-    (Csharpminor.program_of_program p).
+Definition transf_c_program (p: Csyntax.program) : option PPC.program :=
+  match Ctyping.typecheck_program p with
+  | false => None
+  | true =>
+      Some p 
+      @@@ Cshmgen.transl_program
+      @@@ Cminorgen.transl_program
+      @@@ transf_cminor_program
+  end.
 
 (** * Equivalence with whole program transformations *)
 
@@ -126,23 +124,18 @@ Definition transf_cminor_program2 (p: Cminor.program) : option PPC.program :=
   @@@ Stacking.transf_program
   @@@ PPCgen.transf_program.
 
-Definition transf_csharpminor_program2 (p: Csharpminor.program) : option PPC.program :=
-  Some p
-  @@@ Cminorgen.transl_program
-  @@@ transf_cminor_program2.
-
-Lemma transf_partial_program_compose:
-  forall (A B C: Set)
+Lemma map_partial_compose:
+  forall (X A B C: Set)
          (f1: A -> option B) (f2: B -> option C)
-         (p: list (ident * A)),
-  transf_partial_program f1 p @@@ transf_partial_program f2 =
-  transf_partial_program (fun f => f1 f @@@ f2) p.
+         (p: list (X * A)),
+  map_partial f1 p @@@ map_partial f2 =
+  map_partial (fun f => f1 f @@@ f2) p.
 Proof.
   induction p. simpl. auto.
   simpl. destruct a. destruct (f1 a). 
-  simpl. simpl in IHp. destruct (transf_partial_program f1 p).
+  simpl. simpl in IHp. destruct (map_partial f1 p).
   simpl. simpl in IHp. destruct (f2 b).
-  destruct (transf_partial_program f2 l). 
+  destruct (map_partial f2 l). 
   rewrite <- IHp. auto.
   rewrite <- IHp. auto.
   auto.
@@ -150,40 +143,67 @@ Proof.
   simpl. auto.
 Qed.
 
+(*
+Lemma transform_partial_program2_compose:
+  forall (A B C V W X: Set)
+         (f1: A -> option B) (g1: V -> option W)
+         (f2: B -> option C) (g2: W -> option X)
+         (p: program A V),
+  transform_partial_program2 f1 g1 p @@@
+                  (fun p' => transform_partial_program2 f2 g2 p') =
+  transform_partial_program2 (fun x => f1 x @@@ f2) (fun x => g1 x @@@ g2) p.
+Proof.
+  unfold transform_partial_program2; intros.
+  rewrite <- map_partial_compose; simpl.
+  rewrite <- map_partial_compose; simpl.
+  destruct (map_partial f1 (prog_funct p)); simpl; auto.
+  destruct (map_partial g1 (prog_vars p)); simpl; auto.
+  destruct (map_partial f2 l); auto.
+Qed.
+
+Lemma transform_program_partial2_partial:
+  forall (A B V: Set) (f: A -> option B) (p: program A V),
+  transform_partial_program f p =
+  transform_partial_program2 f (fun x => Some x) p.
+Proof.
+  intros. unfold transform_partial_program, transform_partial_program2.
+  rewrite map_partial_identity. auto.
+Qed.
+
+Lemma apply_partial_transf_program:
+  forall (A B V: Set) (f: A -> option B) (x: option (program A V)),
+  x @@@ (fun p => transform_partial_program f p) =
+  x @@@ (fun p => transform_partial_program2 f (fun x => Some x) p).
+Proof.
+  intros. unfold apply_partial. 
+  destruct x. apply transform_program_partial2_partial. auto.
+Qed.
+*)
 Lemma transform_partial_program_compose:
-  forall (A B C: Set)
+  forall (A B C V: Set)
          (f1: A -> option B) (f2: B -> option C)
-         (p: program A),
+         (p: program A V),
   transform_partial_program f1 p @@@
-                        (fun p' => transform_partial_program f2 p') =
+                       (fun p' => transform_partial_program f2 p') =
   transform_partial_program (fun f => f1 f @@@ f2) p.
 Proof.
   unfold transform_partial_program; intros.
-  rewrite <- transf_partial_program_compose. simpl. 
-  destruct (transf_partial_program f1 (prog_funct p)); simpl.
+  rewrite <- map_partial_compose. simpl. 
+  destruct (map_partial f1 (prog_funct p)); simpl.
   auto. auto. 
 Qed.
 
-Lemma transf_program_partial_total:
-  forall (A B: Set) (f: A -> B) (l: list (ident * A)),
-  Some (AST.transf_program f l) =
-    AST.transf_partial_program (fun x => Some (f x)) l.
-Proof.
-  induction l. simpl. auto.
-  simpl. destruct a. rewrite <- IHl. auto.
-Qed.
-
 Lemma transform_program_partial_total:
-  forall (A B: Set) (f: A -> B) (p: program A),
+  forall (A B V: Set) (f: A -> B) (p: program A V),
   Some (transform_program f p) =
     transform_partial_program (fun x => Some (f x)) p.
 Proof.
   intros. unfold transform_program, transform_partial_program.
-  rewrite <- transf_program_partial_total. auto.
+  rewrite map_partial_total. auto. 
 Qed.
 
 Lemma apply_total_transf_program:
-  forall (A B: Set) (f: A -> B) (x: option (program A)),
+  forall (A B V: Set) (f: A -> B) (x: option (program A V)),
   x @@ (fun p => transform_program f p) =
   x @@@ (fun p => transform_partial_program (fun x => Some (f x)) p).
 Proof.
@@ -219,6 +239,7 @@ Proof.
   reflexivity.
 Qed.
 
+(*
 Lemma transf_csharpminor_program_equiv:
   forall p, transf_csharpminor_program2 p = transf_csharpminor_program p.
 Proof.
@@ -227,22 +248,27 @@ Proof.
   simpl. 
   replace transf_cminor_program2 with transf_cminor_program.
   unfold transf_cminor_program, Cminorgen.transl_program, Cminor.program, PPC.program.
-  apply transform_partial_program_compose. 
+  rewrite apply_partial_transf_program.
+  rewrite transform_partial_program2_compose.
+  reflexivity.
   symmetry. apply extensionality. exact transf_cminor_program_equiv.
 Qed.
+*)
 
 (** * Semantic preservation *)
 
-(** We prove that the [transf_program2] translations preserve semantics.  The proof
-  composes the semantic preservation results for each pass. *)
+(** We prove that the [transf_program] translations preserve semantics.  The proof
+  composes the semantic preservation results for each pass.
+  This establishes the correctness of the whole compiler! *)
 
-Lemma transf_cminor_program2_correct:
+Theorem transf_cminor_program_correct:
   forall p tp t n,
-  transf_cminor_program2 p = Some tp ->
+  transf_cminor_program p = Some tp ->
   Cminor.exec_program p t (Vint n) ->
   PPC.exec_program tp t (Vint n).
 Proof.
   intros until n.
+  rewrite <- transf_cminor_program_equiv.
   unfold transf_cminor_program2.
   simpl. caseEq (RTLgen.transl_program p). intros p1 EQ1. 
   simpl. set (p2 := CSE.transf_program (Constprop.transf_program p1)).
@@ -273,39 +299,19 @@ Proof.
   simpl; intros; discriminate.
 Qed.
 
-Lemma transf_csharpminor_program2_correct:
+Theorem transf_c_program_correct:
   forall p tp t n,
-  transf_csharpminor_program2 p = Some tp ->
-  Csharpminor.exec_program p t (Vint n) ->
+  transf_c_program p = Some tp ->
+  Csem.exec_program p t (Vint n) ->
   PPC.exec_program tp t (Vint n).
 Proof.
-  intros until n; unfold transf_csharpminor_program2; simpl.
-  caseEq (Cminorgen.transl_program p).
-  simpl; intros p1 EQ1 EQ2 EXEC. 
-  apply transf_cminor_program2_correct with p1. auto. 
-  apply Cminorgenproof.transl_program_correct with p. auto.
-  assumption.
-  simpl; intros; discriminate.
-Qed.
-
-(** It follows that the whole compiler is semantic-preserving. *)
-
-Theorem transf_cminor_program_correct:
-  forall p tp t n,
-  transf_cminor_program p = Some tp ->
-  Cminor.exec_program p t (Vint n) ->
-  PPC.exec_program tp t (Vint n).
-Proof.
-  intros. apply transf_cminor_program2_correct with p. 
-  rewrite transf_cminor_program_equiv. assumption. assumption.
-Qed.
-
-Theorem transf_csharpminor_program_correct:
-  forall p tp t n,
-  transf_csharpminor_program p = Some tp ->
-  Csharpminor.exec_program p t (Vint n) ->
-  PPC.exec_program tp t (Vint n).
-Proof.
-  intros. apply transf_csharpminor_program2_correct with p. 
-  rewrite transf_csharpminor_program_equiv. assumption. assumption.
+  intros until n; unfold transf_c_program; simpl.
+  caseEq (Ctyping.typecheck_program p); try congruence; intro.
+  caseEq (Cshmgen.transl_program p); simpl; try congruence; intros p1 EQ1.
+  caseEq (Cminorgen.transl_program p1); simpl; try congruence; intros p2 EQ2. 
+  intros EQ3 SEM.
+  eapply transf_cminor_program_correct; eauto.
+  eapply Cminorgenproof.transl_program_correct; eauto. 
+  eapply Cshmgenproof3.transl_program_correct; eauto.
+  apply Ctyping.typecheck_program_correct; auto.
 Qed.
