backend/CSEproof.v
@@ -765,13 +765,13 @@ Lemma functions_translated:
   forall (v: val) (f: RTL.fundef),
   Genv.find_funct ge v = Some f ->
   Genv.find_funct tge v = Some (transf_fundef f).
-Proof (@Genv.find_funct_transf _ _ transf_fundef prog).
+Proof (@Genv.find_funct_transf _ _ _ transf_fundef prog).
 
 Lemma funct_ptr_translated:
   forall (b: block) (f: RTL.fundef),
   Genv.find_funct_ptr ge b = Some f ->
   Genv.find_funct_ptr tge b = Some (transf_fundef f).
-Proof (@Genv.find_funct_ptr_transf _ _ transf_fundef prog).
+Proof (@Genv.find_funct_ptr_transf _ _ _ transf_fundef prog).
 
 Lemma sig_translated:
   forall (f: RTL.fundef),
